We have two cases to consider; either the triangle has sides $(x, x, x+1)$ or it has sides $(x, x, x-1)$.

Assume the triangle has sides $(x, x, x+1)$. The area of this triangle is $\frac{(x+1)\sqrt{3x^2-2x-1}}{4}$ by Heron's formula. We aim to find when the discriminant is an integer, so letting $\sqrt{3x^2-2x-1}=k$, it follows that $x=\frac{2+2\sqrt{4+3k^2}}{6}$. Clearly $k$ is even.

Letting $l = \sqrt{4+3k^2}$, we get $l^2 - 3k^2 = 4$. Since $k$ is even, $l$ is also even, so we let $(h, m) = (\frac{l}{2}, \frac{k}{2})$. Now we have the Pell equation $h^2 - 3m^2 = 1$.

The first few solutions to this are $(h, m) = (1, 0), (2, 1), (7, 4)$. We notice that if $(h, m)$ is a solution, then so is $(2h+3m, h+2m)$. We can now recursively generate solutions. 

Note that we double step to avoid fractions. This gives us $\begin{bmatrix}
2 & 3\\
1 & 2
\end{bmatrix}^2 = \begin{bmatrix}
7 & 12\\
4 & 7
\end{bmatrix}$, meaning if $(h, m)$ is a solution, so is $(7h+12m, 4h+7m)$.

Similar casework applies for $(x, x, x-1)$.